methods names and code reorganization

managerOnlyUpdates - with changes.dfy
@@ -1,162 +1,3 @@
-function isPublisherOut (publisher : Publisher, ads: map <Publisher, Ad>, publishers : seq<Publisher>) : bool
-        {
-        publisher !in publishers &&
-        publisher !in ads
-        }
-
-        function adsKeysEqualsPublishers (ads: map <Publisher, Ad>, publishers : seq<Publisher>) : bool
-        {
-        (forall p :: p in publishers ==> p in ads) &&
-        (forall p :: p in ads ==> p in publishers)
-        }
-
-        function valuesOfAds (myAds : map<Publisher, Ad>) : set<Ad>
-{
-        set p: Publisher | p in myAds :: myAds[p]
-        }
-
-        function isNoNullPublishers (ads: map <Publisher, Ad>, publishers : seq<Publisher>) : bool
-        requires adsKeysEqualsPublishers(ads, publishers)
-        reads valuesOfAds(ads)
-        {
-        forall p :: p in publishers ==> p != null && ads[p] != null && ads[p].banner != null
-        }
-
-        function isNoNullAds (ads: map <Publisher, Ad>) : bool
-        {
-        forall p :: p in ads ==> ads[p] != null
-        }
-
-        function isNoNullAvailableBanners (availableBanners: seq<Banner>) : bool
-        {
-        forall i :: 0 <= i < |availableBanners| ==> availableBanners[i] != null
-        }
-
-        function isUniqueAvailableBanners (availableBanners: seq<Banner>) : bool
-        {
-        |availableBanners| > 0 ==> availableBanners[0] !in availableBanners[1..]
-        }
-
-        function isPublisherInMap (publisher : Publisher, retAds: map <Publisher, Ad>) : bool
-        {
-        publisher in retAds &&
-        retAds[publisher] != null
-        }
-
-        function checkStartPublishRoomInAvailableBanners(publisher : Publisher, price : int, publishers : seq<Publisher>, retPublishers: seq<Publisher>, ads : map <Publisher, Ad>, retAds: map <Publisher, Ad>, availableBanners : seq<Banner>, retBanners: seq<Banner>) : bool
-        reads valuesOfAds(retAds)
-        { //must add enters here - I don't know the scopes:
-        |availableBanners| > 0 ==> publisher in retPublishers && publisher in retAds && retAds[publisher] != null && retAds[publisher].price == price  && availableBanners[0] == retAds[publisher].banner && retBanners == availableBanners[1..] && availableBanners[0] !in retBanners
-        }
-
-        function checkStartPublishAllListsEmpty (publisher : Publisher, price : int, publishers : seq<Publisher>, retPublishers: seq<Publisher>, ads : map <Publisher, Ad>, retAds: map <Publisher, Ad>, availableBanners : seq<Banner>, retBanners: seq<Banner>) : bool
-        {
-        (|availableBanners| == 0 && |publishers| == 0) ==> publishers == retPublishers && ads == retAds && availableBanners == retBanners && publisher !in publishers && publisher !in ads
-        }
-
-        function checkStartPublishBidAccepted (publisher : Publisher, price : int, publishers : seq<Publisher>, retPublishers: seq<Publisher>, ads : map <Publisher, Ad>, retAds: map <Publisher, Ad>, availableBanners : seq<Banner>, retBanners: seq<Banner>, globalMinPublisher: Publisher) : bool
-        reads valuesOfAds(retAds)
-        reads valuesOfAds(ads)
-        requires forall p :: p in ads ==> ads[p] != null
-        {
-        (|availableBanners| == 0 && |publishers| > 0 && !isPriceLessThanMinPrice(price, ads)) ==> (publisher in retPublishers && isPublisherInMap(publisher, retAds) && retAds[publisher].price == price && availableBanners == retBanners) && (globalMinPublisher !in retPublishers && globalMinPublisher !in retAds && globalMinPublisher in ads && retAds[publisher].banner == ads[globalMinPublisher].banner)
-        }
-
-        function isPriceLessThanMinPrice (price : int, ads: map <Publisher, Ad>) : bool
-        reads valuesOfAds(ads)
-        {
-        forall p :: p in ads && ads[p] != null ==> ads[p].price >= price
-        }
-
-        function checkStartPublishBidNotAccepted (publisher : Publisher, price : int, publishers : seq<Publisher>, retPublishers: seq<Publisher>, ads : map <Publisher, Ad>, retAds: map <Publisher, Ad>, availableBanners : seq<Banner>, retBanners: seq<Banner>) : bool
-        reads valuesOfAds(ads)
-        {
-        (|availableBanners| == 0 && |publishers| > 0 && isPriceLessThanMinPrice(price, ads)) ==> publishers == retPublishers && ads == retAds && availableBanners == retBanners && isPublisherOut(publisher, ads, publishers)
-        }
-
-        function isNoNull (availableBanners: seq<Banner>, publishers : seq<Publisher>, ads : map <Publisher, Ad>)  : bool
-        reads valuesOfAds(ads)
-        requires adsKeysEqualsPublishers(ads, publishers)
-        {
-        isNoNullPublishers(ads,publishers) && isNoNullAds(ads) && isNoNullAvailableBanners(availableBanners)
-        }
-
-        function adExists(adService : AdvertisingService, publisher: Publisher, ads: map <Publisher, Ad>, availableBanners: seq<Banner>) : bool
-        reads valuesOfAds(ads)
-        {
-        isPublisherInMap(publisher, ads) && ads[publisher].banner !in availableBanners
-        }
-
-        function startPublishRequirements (publisher: Publisher, availableBanners: seq<Banner>, publishers : seq<Publisher>, ads : map <Publisher, Ad>)  : bool
-        reads valuesOfAds(ads)
-        {
-        isPublisherOut(publisher, ads, publishers) && adsKeysEqualsPublishers(ads, publishers) && isUniqueAvailableBanners(availableBanners) && adsKeysEqualsPublishers(ads, publishers)
-        }
-
-        function findMinPublisherPreConditions(publishers : seq<Publisher>, ads : map <Publisher, Ad>) : bool
-        reads valuesOfAds(ads)
-        {
-        |publishers| > 0 && forall p :: p in publishers ==> p != null && p in ads && ads[p] != null && ads[p].banner != null && adsKeysEqualsPublishers(ads, publishers) && isNoNullAds(ads)
-        }
-
-        function findMinPublisherPostConditions(retPrice : int, retPublisher : Publisher, publishers : seq<Publisher>, ads : map <Publisher, Ad>) : bool
-        requires forall p :: p in ads ==> ads[p] != null
-        reads valuesOfAds(ads)
-        {
-        retPublisher in ads && retPublisher in publishers && retPublisher != null && ads[retPublisher] != null && ads[retPublisher].banner != null && ads[retPublisher].price == retPrice && forall p :: p in ads ==> ads[p].price >= retPrice
-        }
-
-        function startPublishPostConditions(publisher : Publisher, price : int, publishers : seq<Publisher>, retPublishers: seq<Publisher>, ads : map <Publisher, Ad>, retAds: map <Publisher, Ad>, availableBanners : seq<Banner>, retBanners: seq<Banner>, globalMinPublisher: Publisher) : bool
-        reads valuesOfAds(retAds)
-        reads valuesOfAds(ads)
-        requires forall p :: p in ads ==> ads[p] != null
-        {
-        checkStartPublishRoomInAvailableBanners(publisher, price, publishers, retPublishers, ads, retAds, availableBanners, retBanners)
-        && checkStartPublishBidNotAccepted(publisher, price, publishers, retPublishers, ads, retAds, availableBanners, retBanners)
-        && checkStartPublishBidAccepted(publisher, price, publishers, retPublishers, ads, retAds, availableBanners, retBanners, globalMinPublisher)
-        && checkStartPublishAllListsEmpty(publisher, price, publishers, retPublishers, ads, retAds, availableBanners, retBanners)
-        }
-
-        function removePublisherInvPublisherOut(index: int, publishers: seq<Publisher>, newPublishers: seq<Publisher>, publisher: Publisher) : bool
-        {
-        0 <= index <= |publishers| && publisher !in newPublishers
-        }
-
-        function removePublisherInvRestIn(index: int, publishers: seq<Publisher>, newPublishers: seq<Publisher>, publisher: Publisher) : bool
-        requires index <= |publishers|
-        {
-        forall i :: 0 <= i < index && publishers[i] != publisher ==> publishers[i] in newPublishers
-        }
-
-
-        function findMinPublisherInvDataStructuresOk(minPrice: int, ads : map <Publisher, Ad>, index: int, publishers: seq<Publisher>, minPublisher: Publisher) : bool
-        reads valuesOfAds(ads)
-        {
-        forall p :: p in publishers ==> p in ads && minPublisher in ads && ads[minPublisher] != null && ads[minPublisher].price == minPrice && minPublisher in publishers
-        }
-
-        function findMinPublisherInvMinPriceCorrect(minPrice: int, ads : map <Publisher, Ad>, index: int, publishers: seq<Publisher>, minPublisher: Publisher) : bool
-        requires isNoNullAds(ads)
-        requires adsKeysEqualsPublishers(ads, publishers)
-        reads valuesOfAds(ads)
-        {
-        0 <= index <= |publishers| && minPublisher in ads && forall i :: 0 <= i < index ==> minPrice <= ads[publishers[i]].price && isNoNullAds(ads)
-        }
-
-
-        function bannerRemovedInvariant(banner : Banner, retBanners : seq<Banner>, availableBanners : seq<Banner>) : bool
-        {
-        banner !in retBanners &&
-        forall b :: b in availableBanners && b != banner ==> b in retBanners
-        }
-
-        function adRemovedInvariant(publisher : Publisher, retAds : map <Publisher, Ad>, ads : map <Publisher, Ad>) : bool
-        {
-        publisher !in retAds &&
-        forall p :: p in ads && p != publisher ==> p in retAds && retAds[p] == ads[p]
-        }
-
-
 class AdvertisingManager {
 
     var availableBanners: seq<Banner>;
@@ -244,9 +85,8 @@ class AdvertisingService
         var index := 0;
         var newBanners : seq<Banner> := [];
         while (index < |availableBanners|)
-            decreases |availableBanners| - index
-        invariant 0 <= index <= |availableBanners| && banner !in newBanners
-        invariant forall i :: 0 <= i < index && availableBanners[i] != banner ==> availableBanners[i] in newBanners
+        decreases |availableBanners| - index
+        invariant removeBannerLoopInvariant(index, availableBanners, newBanners, banner)
         {
             if (availableBanners[index] != banner)
             {
@@ -264,15 +104,13 @@ class AdvertisingService
     }
 
     method removePublisher(publisher : Publisher, publishers : seq<Publisher>) returns (retPublishers : seq<Publisher>)
-    ensures publisher !in retPublishers
-    ensures forall p :: p in publishers && p != publisher ==> p in retPublishers
+    ensures removePublisherInvariant(publisher, publishers, retPublishers)
     {
         var index := 0;
         var newPublishers : seq<Publisher> := [];
         while (index < |publishers|)
-            decreases |publishers| - index
-        invariant removePublisherInvPublisherOut(index, publishers, newPublishers, publisher)
-        invariant removePublisherInvRestIn(index, publishers, newPublishers, publisher)
+        decreases |publishers| - index
+        invariant removePublisherLoopInvariant(index, publishers, newPublishers, publisher)
         {
             if (publishers[index] != publisher)
             {
@@ -285,44 +123,39 @@ class AdvertisingService
     }
 
     method addPublisher (publisher : Publisher, publishers : seq<Publisher>) returns (retPublishers : seq<Publisher>)
-    ensures publisher in retPublishers
-    ensures forall p :: p in publishers ==> p in retPublishers
+    ensures addPublisherInvariant(publisher, publishers, retPublishers)	
     {
         return publishers + [publisher];
     }
 
     method addAd (publisher : Publisher, price : int, banner : Banner, ads : map <Publisher, Ad>) returns (retAds : map <Publisher, Ad>)
     requires banner != null;
-    ensures isPublisherInMap(publisher, retAds)
-    ensures retAds[publisher].price == price && retAds[publisher].banner == banner
+    ensures addAdInvariant(publisher, price, banner, retAds)
     {
         var newAd : Ad := new Ad(banner, price);
         return ads[publisher := newAd];
     }
 
     method popFirstBanner(banners : seq<Banner>) returns (retBanners : seq<Banner>)
-    requires |banners| > 0
-    requires banners[0] !in banners[1..]
-    ensures banners[0] !in retBanners
-    ensures retBanners == banners[1..]
+    requires |banners| > 0 && banners[0] !in banners[1..]
+    // requires banners[0] !in banners[1..]
+    ensures banners[0] !in retBanners && retBanners == banners[1..]
+    // ensures retBanners == banners[1..]
     {
         return banners[1..];
     }
 
     method findMinPublisher(publishers : seq<Publisher>, ads : map <Publisher, Ad>) returns (retPublisher : Publisher, retPrice : int)
-    requires findMinPublisherPreConditions(publishers, ads)
-    requires forall p :: p in ads ==> ads[p] != null
-    ensures findMinPublisherPostConditions(retPrice, retPublisher, publishers, ads)
+    requires findMinPublisherRequirements(publishers, ads)
+    ensures minPublisherFound(retPrice, retPublisher, publishers, ads)
     {
         var minPublisher := publishers[0];
         var minPrice := ads[minPublisher].price;
 
         var index := 1;
         while (index < |publishers|)
-            decreases |publishers| - index
-        invariant findMinPublisherInvDataStructuresOk(minPrice, ads, index, publishers, minPublisher)
-        invariant findMinPublisherInvMinPriceCorrect(minPrice, ads, index, publishers, minPublisher)
-        // checkInvariantFindMinPublisher(index, publishers, ads,minPublisher, minPrice);
+        decreases |publishers| - index
+        invariant findMinPublisherLoopInvariant(minPrice, ads, index, publishers, minPublisher)
         {
             var curPrice := ads[publishers[index]].price;
             if (curPrice < minPrice)
@@ -339,8 +172,7 @@ class AdvertisingService
     modifies this
     requires startPublishRequirements(publisher, availableBanners, publishers, ads)
     requires isNoNull (availableBanners, publishers, ads)
-    ensures startPublishPostConditions(publisher, price, publishers, retPublishers, ads, retAds, availableBanners, retBanners, globalMinPublisher);
-
+    ensures startPublishInvariant(publisher, price, publishers, retPublishers, ads, retAds, availableBanners, retBanners, globalMinPublisher);
     {
         var newPublishers : seq<Publisher> := publishers;
         var newAds : map <Publisher, Ad> := ads;
@@ -396,13 +228,238 @@ class Ad
     constructor(bannerArg : Banner, priceArg : int)
     modifies this;
     requires bannerArg != null;
-    ensures banner == bannerArg;
-    ensures price == priceArg;
+    ensures banner == bannerArg && price == priceArg;
     {
         banner := bannerArg;
         price := priceArg;
     }
 }
+
+function isPublishing (publisher : Publisher, ads: map <Publisher, Ad>, publishers : seq<Publisher>) : bool
+		{
+        publisher !in publishers &&
+        publisher !in ads
+        }
+
+        function adsKeysEqualsPublishers (ads: map <Publisher, Ad>, publishers : seq<Publisher>) : bool
+        {
+        (forall p :: p in publishers ==> p in ads) &&
+        (forall p :: p in ads ==> p in publishers)
+        }
+
+        function valuesOfAds (myAds : map<Publisher, Ad>) : set<Ad>
+        {
+        set p: Publisher | p in myAds :: myAds[p]
+        }
+
+        function isNoNullPublishers (ads: map <Publisher, Ad>, publishers : seq<Publisher>) : bool
+        requires adsKeysEqualsPublishers(ads, publishers)
+        reads valuesOfAds(ads)
+        {
+        forall p :: p in publishers ==> p != null && ads[p] != null && ads[p].banner != null
+        }
+
+        function isNoNullAds (ads: map <Publisher, Ad>) : bool
+        {
+        forall p :: p in ads ==> ads[p] != null
+        }
+
+        function isNoNullAvailableBanners (availableBanners: seq<Banner>) : bool
+        {
+        forall i :: 0 <= i < |availableBanners| ==> availableBanners[i] != null
+        }
+
+        function isUniqueAvailableBanners (availableBanners: seq<Banner>) : bool
+        {
+        |availableBanners| > 0 ==> availableBanners[0] !in availableBanners[1..]
+        }
+
+        function isPublisherInAds (publisher : Publisher, retAds: map <Publisher, Ad>) : bool
+		{
+        publisher in retAds &&
+        retAds[publisher] != null
+        }
+
+        function startPublishWithAvailableBanner(publisher : Publisher, price : int, publishers : seq<Publisher>, retPublishers: seq<Publisher>, ads : map <Publisher, Ad>, retAds: map <Publisher, Ad>, availableBanners : seq<Banner>, retBanners: seq<Banner>) : bool
+		reads valuesOfAds(retAds)
+        {
+        |availableBanners| > 0 ==> publisher in retPublishers && 
+		publisher in retAds && 
+		retAds[publisher] != null && 
+		retAds[publisher].price == price  && 
+		availableBanners[0] == retAds[publisher].banner && 
+		retBanners == availableBanners[1..] && 
+		availableBanners[0] !in retBanners
+        }
+
+        function startPublishEmptyList (publisher : Publisher, price : int, publishers : seq<Publisher>, retPublishers: seq<Publisher>, ads : map <Publisher, Ad>, retAds: map <Publisher, Ad>, availableBanners : seq<Banner>, retBanners: seq<Banner>) : bool
+		{
+        (|availableBanners| == 0 && 
+		|publishers| == 0) ==> publishers == retPublishers && 
+		ads == retAds && 
+		availableBanners == retBanners && 
+		publisher !in publishers && 
+		publisher !in ads
+        }
+
+        function publishingStarted (publisher : Publisher, price : int, publishers : seq<Publisher>, retPublishers: seq<Publisher>, ads : map <Publisher, Ad>, retAds: map <Publisher, Ad>, availableBanners : seq<Banner>, retBanners: seq<Banner>, globalMinPublisher: Publisher) : bool
+		reads valuesOfAds(retAds)
+        reads valuesOfAds(ads)
+        requires forall p :: p in ads ==> ads[p] != null
+        {
+        (|availableBanners| == 0 && 
+		|publishers| > 0 && 
+		!isPriceLessThanMinPrice(price, ads)) ==> (publisher in retPublishers && 
+		isPublisherInAds(publisher, retAds) && 
+		retAds[publisher].price == price && 
+		availableBanners == retBanners) && 
+		(globalMinPublisher !in retPublishers && 
+		globalMinPublisher !in retAds && 
+		globalMinPublisher in ads && 
+		retAds[publisher].banner == ads[globalMinPublisher].banner)
+        }
+
+        function isPriceLessThanMinPrice (price : int, ads: map <Publisher, Ad>) : bool
+        reads valuesOfAds(ads)
+        {
+        forall p :: p in ads && 
+		ads[p] != null ==> ads[p].price >= price
+        }
+
+        function publishingNotStarted (publisher : Publisher, price : int, publishers : seq<Publisher>, retPublishers: seq<Publisher>, ads : map <Publisher, Ad>, retAds: map <Publisher, Ad>, availableBanners : seq<Banner>, retBanners: seq<Banner>) : bool
+		reads valuesOfAds(ads)
+        {
+        (|availableBanners| == 0 && 
+		|publishers| > 0 && 
+		isPriceLessThanMinPrice(price, ads)) ==> publishers == retPublishers && 
+		ads == retAds && availableBanners == retBanners && 
+		isPublishing(publisher, ads, publishers)
+        }
+
+        function isNoNull (availableBanners: seq<Banner>, publishers : seq<Publisher>, ads : map <Publisher, Ad>)  : bool
+        reads valuesOfAds(ads)
+        requires adsKeysEqualsPublishers(ads, publishers)
+        {
+        isNoNullPublishers(ads,publishers) && 
+		isNoNullAds(ads) && 
+		isNoNullAvailableBanners(availableBanners)
+        }
+
+        function adExists(adService : AdvertisingService, publisher: Publisher, ads: map <Publisher, Ad>, availableBanners: seq<Banner>) : bool
+        reads valuesOfAds(ads)
+        {
+        isPublisherInAds(publisher, ads) && 
+		ads[publisher].banner !in availableBanners
+        }
+
+        function startPublishRequirements (publisher: Publisher, availableBanners: seq<Banner>, publishers : seq<Publisher>, ads : map <Publisher, Ad>)  : bool
+        reads valuesOfAds(ads)
+        {
+        isPublishing(publisher, ads, publishers) && 
+		adsKeysEqualsPublishers(ads, publishers) && 
+		isUniqueAvailableBanners(availableBanners) && 
+		adsKeysEqualsPublishers(ads, publishers)
+        }
+
+        function findMinPublisherRequirements(publishers : seq<Publisher>, ads : map <Publisher, Ad>) : bool
+		reads valuesOfAds(ads)
+        {
+        |publishers| > 0 && 
+		forall p :: p in publishers ==> p != null && 
+		p in ads && ads[p] != null && 
+		ads[p].banner != null && 
+		adsKeysEqualsPublishers(ads, publishers) && 
+		isNoNullAds(ads) &&
+		(forall p :: p in ads ==> ads[p] != null)
+        }
+
+        function minPublisherFound(retPrice : int, retPublisher : Publisher, publishers : seq<Publisher>, ads : map <Publisher, Ad>) : bool
+		requires findMinPublisherRequirements(publishers, ads)
+        reads valuesOfAds(ads)
+        {
+        retPublisher in ads && 
+		retPublisher in publishers && 
+		retPublisher != null && 
+		ads[retPublisher] != null && 
+		ads[retPublisher].banner != null && 
+		ads[retPublisher].price == retPrice && 
+		forall p :: p in ads ==> ads[p].price >= retPrice
+        }
+
+        function startPublishInvariant(publisher : Publisher, price : int, publishers : seq<Publisher>, retPublishers: seq<Publisher>, ads : map <Publisher, Ad>, retAds: map <Publisher, Ad>, availableBanners : seq<Banner>, retBanners: seq<Banner>, globalMinPublisher: Publisher) : bool
+        reads valuesOfAds(retAds)
+        reads valuesOfAds(ads)
+        requires forall p :: p in ads ==> ads[p] != null
+        {
+        startPublishWithAvailableBanner(publisher, price, publishers, retPublishers, ads, retAds, availableBanners, retBanners) && 
+		publishingNotStarted(publisher, price, publishers, retPublishers, ads, retAds, availableBanners, retBanners) && 
+		publishingStarted(publisher, price, publishers, retPublishers, ads, retAds, availableBanners, retBanners, globalMinPublisher) && 
+		startPublishEmptyList(publisher, price, publishers, retPublishers, ads, retAds, availableBanners, retBanners)
+        }
+
+		function removePublisherLoopInvariant(index: int, publishers: seq<Publisher>, newPublishers: seq<Publisher>, publisher: Publisher) : bool
+		{
+        0 <= index <= |publishers| && 
+		publisher !in newPublishers && 
+		forall i :: 0 <= i < index && 
+		publishers[i] != publisher ==> publishers[i] in newPublishers
+        }
+
+
+		function findMinPublisherLoopInvariant(minPrice: int, ads : map <Publisher, Ad>, index: int, publishers: seq<Publisher>, minPublisher: Publisher) : bool
+        requires isNoNullAds(ads)
+        requires adsKeysEqualsPublishers(ads, publishers)
+        reads valuesOfAds(ads)
+        {
+        forall p :: p in publishers ==> p in ads && 
+		minPublisher in ads && 
+		ads[minPublisher] != null && 
+		ads[minPublisher].price == minPrice && 
+		minPublisher in publishers && 
+		0 <= index <= |publishers| && 
+		minPublisher in ads && 
+		forall i :: 0 <= i < index ==> minPrice <= ads[publishers[i]].price && 
+		isNoNullAds(ads)
+        }
+
+        function bannerRemovedInvariant(banner : Banner, retBanners : seq<Banner>, availableBanners : seq<Banner>) : bool
+        {
+        banner !in retBanners &&
+        forall b :: b in availableBanners && b != banner ==> b in retBanners
+        }
+
+        function adRemovedInvariant(publisher : Publisher, retAds : map <Publisher, Ad>, ads : map <Publisher, Ad>) : bool
+        {
+        publisher !in retAds &&
+        forall p :: p in ads && p != publisher ==> p in retAds && retAds[p] == ads[p]
+        }
+
+		function removePublisherInvariant(publisher : Publisher, publishers : seq<Publisher>, retPublishers : seq<Publisher>) : bool
+		{
+		publisher !in retPublishers && 
+		forall p :: p in publishers && 
+		p != publisher ==> p in retPublishers
+		}
+
+		function addPublisherInvariant(publisher : Publisher, publishers : seq<Publisher>, retPublishers : seq<Publisher>) : bool
+		{
+		publisher in retPublishers && 
+		forall p :: p in publishers ==> p in retPublishers
+		}
+
+		function addAdInvariant(publisher : Publisher, price : int, banner : Banner, retAds : map <Publisher, Ad>) : bool
+		reads valuesOfAds(retAds)
+		{
+		isPublisherInAds(publisher, retAds) && 
+		retAds[publisher].price == price && 
+		retAds[publisher].banner == banner
+		}
+
+		function removeBannerLoopInvariant(index: int, availableBanners: seq<Banner>, newBanners: seq<Banner>, banner: Banner) : bool
+		{
+		0 <= index <= |availableBanners| && banner !in newBanners && forall i :: 0 <= i < index && availableBanners[i] != banner ==> availableBanners[i] in newBanners
+		}
+
 
 
 
